cleanup: rename "SplitPredicate" to "SplitFunction"

src/lib/state/DY.Lib.State.Tagged.fst
@@ -2,7 +2,7 @@ module DY.Lib.State.Tagged
 
 open Comparse
 open DY.Core
-open DY.Lib.SplitPredicate
+open DY.Lib.SplitFunction
 open DY.Lib.Comparse.Glue
 open DY.Lib.Comparse.Parsers
 
@@ -40,14 +40,14 @@ type local_bytes_state_predicate {|crypto_invariants|} = {
   ;
 }
 
-let split_local_bytes_state_predicate_func {|crypto_invariants|} : split_predicate_input_values = {
+let split_local_bytes_state_predicate_func {|crypto_invariants|} : split_function_input_values = {
   tagged_data_t = trace & principal & state_id & bytes;
   tag_t = string;
   encoded_tag_t = string;
   raw_data_t = trace & principal & state_id & bytes;
   output_t = prop;
 
-  default_global_pred = (fun tr prin sess_id sess_content -> False);
+  default_global_fun = (fun tr prin sess_id sess_content -> False);
 
   decode_tagged_data = (fun (tr, prin, sess_id, sess_content) -> (
     match parse tagged_state sess_content with
@@ -58,30 +58,30 @@ let split_local_bytes_state_predicate_func {|crypto_invariants|} : split_predica
   encode_tag = (fun s -> s);
   encode_tag_inj = (fun l1 l2 -> ());
 
-  local_pred = local_bytes_state_predicate;
-  global_pred = trace -> principal -> state_id -> bytes -> prop;
+  local_fun = local_bytes_state_predicate;
+  global_fun = trace -> principal -> state_id -> bytes -> prop;
 
-  apply_local_pred = (fun spred (tr, prin, sess_id, content) ->
+  apply_local_fun = (fun spred (tr, prin, sess_id, content) ->
     spred.pred tr prin sess_id content
   );
-  apply_global_pred = (fun spred (tr, prin, sess_id, content) ->
+  apply_global_fun = (fun spred (tr, prin, sess_id, content) ->
     spred tr prin sess_id content
   );
-  mk_global_pred = (fun spred -> fun tr prin sess_id content ->
+  mk_global_fun = (fun spred -> fun tr prin sess_id content ->
     spred (tr, prin, sess_id, content)
   );
-  apply_mk_global_pred = (fun spred x -> ());
+  apply_mk_global_fun = (fun spred x -> ());
 }
 
 val has_local_bytes_state_predicate: protocol_invariants -> (string & local_bytes_state_predicate) -> prop
 let has_local_bytes_state_predicate invs (tag, spred) =
-  has_local_pred split_local_bytes_state_predicate_func (state_pred) (tag, spred)
+  has_local_fun split_local_bytes_state_predicate_func (state_pred) (tag, spred)
 
 (*** Global tagged state predicate builder ***)
 
 val mk_global_local_bytes_state_predicate: {|crypto_invariants|} -> list (string & local_bytes_state_predicate) -> trace -> principal -> state_id -> bytes -> prop
 let mk_global_local_bytes_state_predicate #cinvs l =
-  mk_global_pred split_local_bytes_state_predicate_func l
+  mk_global_fun split_local_bytes_state_predicate_func l
 
 val mk_global_local_bytes_state_predicate_correct: invs:protocol_invariants -> lpreds:list (string & local_bytes_state_predicate) -> Lemma
   (requires
@@ -91,7 +91,7 @@ val mk_global_local_bytes_state_predicate_correct: invs:protocol_invariants -> l
   (ensures for_allP (has_local_bytes_state_predicate invs) lpreds)
 let mk_global_local_bytes_state_predicate_correct invs lpreds =
   for_allP_eq (has_local_bytes_state_predicate invs) lpreds;
-  FStar.Classical.forall_intro_2 (FStar.Classical.move_requires_2 (mk_global_pred_correct split_local_bytes_state_predicate_func lpreds))
+  FStar.Classical.forall_intro_2 (FStar.Classical.move_requires_2 (mk_global_fun_correct split_local_bytes_state_predicate_func lpreds))
 
 val mk_global_local_bytes_state_predicate_later:
   cinvs:crypto_invariants -> lpreds:list (string & local_bytes_state_predicate) ->
@@ -99,9 +99,9 @@ val mk_global_local_bytes_state_predicate_later:
   (requires mk_global_local_bytes_state_predicate lpreds tr1 prin sess_id full_content /\ tr1 <$ tr2)
   (ensures mk_global_local_bytes_state_predicate lpreds tr2 prin sess_id full_content)
 let mk_global_local_bytes_state_predicate_later cinvs lpreds tr1 tr2 prin sess_id full_content =
-  mk_global_pred_eq split_local_bytes_state_predicate_func lpreds (tr1, prin, sess_id, full_content);
-  mk_global_pred_eq split_local_bytes_state_predicate_func lpreds (tr2, prin, sess_id, full_content);
-  introduce forall lpred content. split_local_bytes_state_predicate_func.apply_local_pred lpred (tr1, prin, sess_id, content) ==> split_local_bytes_state_predicate_func.apply_local_pred lpred (tr2, prin, sess_id, content) with (
+  mk_global_fun_eq split_local_bytes_state_predicate_func lpreds (tr1, prin, sess_id, full_content);
+  mk_global_fun_eq split_local_bytes_state_predicate_func lpreds (tr2, prin, sess_id, full_content);
+  introduce forall lpred content. split_local_bytes_state_predicate_func.apply_local_fun lpred (tr1, prin, sess_id, content) ==> split_local_bytes_state_predicate_func.apply_local_fun lpred (tr2, prin, sess_id, content) with (
     introduce _ ==> _ with _. lpred.pred_later tr1 tr2 prin sess_id content
   );
   match split_local_bytes_state_predicate_func.decode_tagged_data (tr1, prin, sess_id, full_content) with
@@ -115,10 +115,10 @@ val mk_global_local_bytes_state_predicate_knowable:
   (requires mk_global_local_bytes_state_predicate lpreds tr prin sess_id full_content)
   (ensures is_knowable_by (principal_state_label prin sess_id) tr full_content)
 let mk_global_local_bytes_state_predicate_knowable cinvs lpreds tr prin sess_id full_content =
-  mk_global_pred_eq split_local_bytes_state_predicate_func lpreds (tr, prin, sess_id, full_content);
+  mk_global_fun_eq split_local_bytes_state_predicate_func lpreds (tr, prin, sess_id, full_content);
   match split_local_bytes_state_predicate_func.decode_tagged_data (tr, prin, sess_id, full_content) with
   | Some (tag, (_, _, _, content)) -> (
-    match find_local_pred split_local_bytes_state_predicate_func lpreds tag with
+    match find_local_fun split_local_bytes_state_predicate_func lpreds tag with
     | Some lpred -> (
       lpred.pred_knowable tr prin sess_id content;
       serialize_parse_inv_lemma tagged_state full_content;
