src/lib/utils/DY.Lib.SplitFunction.fst
@@ -1,0 +1,333 @@
+module DY.Lib.SplitFunction
+
+open FStar.List.Tot
+
+#set-options "--fuel 1 --ifuel 1"
+
+/// This module defines a library to create a global function from several independent local functions,
+/// also called the "split function methodology".
+///
+/// DY* proofs rely on global protocol invariants composed of functions and predicates
+/// (e.g. what protocol participants are allowed to store, are allowed to sign, or how a usage evolves throughs KDFs),
+/// that must be preserved by each step of the protocol.
+/// The practice of defining this global protocol invariant monolithically somewhere has a few drawbacks:
+/// - it does not allows the user to do modular proofs,
+///   as many unrelated functions and predicates are put in the same place
+/// - when modifying the global invariants for some sub-component,
+///   other unrelated sub-components will need to be re-checked
+///   (because the local invariant they depend on has changed)
+///   (and their proof might fail if the SMT gods are angry!)
+/// - it makes it difficult to create reusable components
+///   (such as a generic state to store private keys)
+///
+/// With this module, we can create a global function from several independent local functions (see mk_global_fun).
+/// Then, proofs of theorems will take as parameter some global function,
+/// with the precondition that it contains a specific local function (see has_local_fun).
+/// In this way, proofs will work for any global function
+/// as long as it contains the relevant local function.
+/// (This is in contrast to proofs reyling on
+/// a monolithic global function
+/// that is defined at the top of a file (using val and let).)
+///
+/// This solves all the problems mentioned above:
+/// functions are defined (locally) where they belong,
+/// proofs are modular because they only depend on
+/// the relevant local function being contained in the global function
+/// (a property that is not affected by other unrelated local functions).
+///
+/// Under the hood, the split function methodology
+/// is simply factorizing out a common pattern we see
+/// when writing monolithic global functions.
+/// Indeed, such a monolithic global function usually
+/// - first disambiguate to which local function its input belong to
+/// - then dispatch the input to that local function, maybe after some modifications.
+/// In practice, it may look like this:
+/// let global_function param1 param2 param3 ... =
+///   // First detect in which sub-component we are in
+///   let tag = ... in
+///   // then dispatch to the corresponding local function
+///   match tag with
+///   | ... -> local_fun1 ...
+///   | ... -> local_fun2 ...
+///   ...
+/// The tag may be obtained in different ways,
+/// for example with the key usage (e.g. for a signature function, see DY.Core.Bytes.Type.usage),
+/// or because some messages are tagged
+/// (e.g. the state content in a state function or the signature input in signature function).
+/// How to obtain this tag is not always trivial,
+/// it is actually a core argument in the proof of
+/// why it is secure to deploy different sub-components in parallel.
+///
+/// The split function methodology can be used to implement horizontal composition:
+/// as long as we can find a way to disambiguate the composed protocols (using the tag),
+/// we can easily construct a global function implementing this horizontal composition.
+
+/// The parameters of the split function methodology.
+
+noeq type split_function_input_values = {
+  // Input type for the global function
+  tagged_data_t: Type;
+
+  // Two types of tag, that are related using `encode_tag`:
+  // the tag type that we use to define the global function,
+  // and the tag type that we obtain when decoding the global function input.
+  // Having different types may be handy in some situations.
+  tag_t: Type;
+  encoded_tag_t: eqtype;
+
+  // Input type for the local functions
+  raw_data_t: Type;
+
+  output_t: Type;
+
+  // We can decode the global function input
+  // into an encoded tag and a local function input
+  decode_tagged_data: tagged_data_t -> Tot (option (encoded_tag_t & raw_data_t));
+
+  // We can encode the tag, and this encoding must be injective.
+  encode_tag: tag_t -> encoded_tag_t;
+  encode_tag_inj: l1:tag_t -> l2:tag_t -> Lemma
+    (requires encode_tag l1 == encode_tag l2)
+    (ensures l1 == l2)
+  ;
+
+  // Types for the local functions and the global function
+  local_fun: Type;
+  global_fun: Type;
+
+  default_global_fun: global_fun;
+
+  // Apply a local function to its input
+  apply_local_fun: local_fun -> raw_data_t -> output_t;
+  // Apply the global function to its input
+  apply_global_fun: global_fun -> tagged_data_t -> output_t;
+  // Create a global function
+  mk_global_fun: (tagged_data_t -> output_t) -> global_fun;
+  // Correctness theorem on creating and applying a global function
+  apply_mk_global_fun: bare:(tagged_data_t -> output_t) -> x:tagged_data_t -> Lemma
+    (apply_global_fun (mk_global_fun bare) x == bare x);
+}
+
+/// Do a global function contain some given local function with some tag?
+/// This will be a crucial precondition for the correctness theorem `local_eq_global_lemma`.
+
+val has_local_fun: func:split_function_input_values -> func.global_fun -> (func.tag_t & func.local_fun) -> prop
+let has_local_fun func gfun (the_tag, lfun) =
+  forall tagged_data.
+    match func.decode_tagged_data tagged_data with
+    | Some (tag, raw_data) ->
+      tag == func.encode_tag the_tag ==> (func.apply_global_fun gfun tagged_data == func.apply_local_fun lfun raw_data)
+    | None -> True
+
+val find_local_fun: func:split_function_input_values -> list (func.tag_t & func.local_fun) -> func.encoded_tag_t -> option func.local_fun
+let rec find_local_fun func l tag =
+  match l with
+  | [] -> None
+  | (the_tag, lfun)::t -> (
+    if tag = func.encode_tag the_tag then
+      Some lfun
+    else
+      find_local_fun func t tag
+  )
+
+val mk_global_fun_aux: func:split_function_input_values -> list (func.tag_t & func.local_fun) -> func.tagged_data_t -> func.output_t
+let mk_global_fun_aux func l tagged_data =
+  match func.decode_tagged_data tagged_data with
+  | Some (tag, raw_data) -> (
+    match find_local_fun func l tag with
+    | Some lfun -> func.apply_local_fun lfun raw_data
+    | None -> func.apply_global_fun func.default_global_fun tagged_data
+  )
+  | None -> func.apply_global_fun func.default_global_fun tagged_data
+
+/// Given a list of tags and local functions, create the global function.
+
+[@@"opaque_to_smt"]
+val mk_global_fun: func:split_function_input_values -> list (func.tag_t & func.local_fun) -> func.global_fun
+let mk_global_fun func l =
+  func.mk_global_fun (mk_global_fun_aux func l)
+
+val find_local_fun_wrong_tag:
+  func:split_function_input_values ->
+  the_tag:func.tag_t -> l:list (func.tag_t & func.local_fun) -> tag:func.encoded_tag_t ->
+  Lemma
+  (requires ~(List.Tot.memP the_tag (List.Tot.map fst l)))
+  (ensures (
+    tag == func.encode_tag the_tag ==> (find_local_fun func l tag == None)
+  ))
+let rec find_local_fun_wrong_tag func the_tag l tag =
+  match l with
+  | [] -> ()
+  | (tag', _)::t -> (
+    FStar.Classical.move_requires_2 func.encode_tag_inj the_tag tag';
+    find_local_fun_wrong_tag func the_tag t tag
+  )
+
+val disjointP: #a:Type -> list a -> list a -> prop
+let rec disjointP #a l1 l2 =
+  match l2 with
+  | [] -> True
+  | h2::t2 ->
+    ~(List.Tot.memP h2 l1) /\ disjointP l1 t2
+
+val disjointP_move:
+  #a:Type ->
+  l1:list a -> x:a -> l2:list a ->
+  Lemma
+  (requires disjointP l1 l2 /\ ~(List.Tot.memP x l2))
+  (ensures disjointP (l1 @ [x]) l2)
+let rec disjointP_move #a l1 x l2 =
+  match l2 with
+  | [] -> ()
+  | h2::t2 ->
+    disjointP_move l1 x t2;
+    List.Tot.append_memP l1 [x] h2;
+    assert_norm(List.Tot.memP h2 [x] <==> h2 == x)
+
+val find_local_fun_move:
+  func:split_function_input_values ->
+  lfuns1:list (func.tag_t & func.local_fun) -> x:(func.tag_t & func.local_fun) -> lfuns2:list (func.tag_t & func.local_fun) ->
+  tag:func.encoded_tag_t ->
+  Lemma
+  (ensures
+    (
+      match find_local_fun func lfuns1 tag with
+      | Some lfun -> Some lfun
+      | None -> find_local_fun func (x::lfuns2) tag
+    ) == (
+      match find_local_fun func (lfuns1 @ [x]) tag with
+      | Some lfun -> Some lfun
+      | None -> find_local_fun func lfuns2 tag
+    )
+  )
+let rec find_local_fun_move func lfuns1 (the_tag, the_sfun) lfuns2 tag =
+  match lfuns1 with
+  | [] -> ()
+  | (h_tag, h_sfun)::t ->
+    find_local_fun_move func t (the_tag, the_sfun) lfuns2 tag
+
+val memP_map:
+  #a:Type -> #b:Type ->
+  f:(a -> b) -> l:list a -> x:a ->
+  Lemma
+  (requires List.Tot.memP x l)
+  (ensures List.Tot.memP (f x) (List.Tot.map f l))
+let rec memP_map #a #b f l x =
+  match l with
+  | [] -> ()
+  | h::t ->
+    introduce x =!= h ==> List.Tot.memP (f x) (List.Tot.map f t)
+    with _. memP_map f t x
+
+val mk_global_fun_correct_aux:
+  func:split_function_input_values -> gfun:(func.encoded_tag_t -> option func.local_fun) -> lfuns1:list (func.tag_t & func.local_fun) -> lfuns2:list (func.tag_t & func.local_fun) -> the_tag:func.tag_t -> lfun:func.local_fun -> tag:func.encoded_tag_t ->
+  Lemma
+  (requires
+    (forall tag. gfun tag == (
+        match find_local_fun func lfuns1 tag with
+        | Some lfun -> Some lfun
+        | None -> (
+          match find_local_fun func lfuns2 tag with
+          | Some lfun -> Some lfun
+          | None -> None
+        )
+      )
+    ) /\
+    List.Tot.no_repeats_p (List.Tot.map fst lfuns2) /\
+    disjointP (List.Tot.map fst lfuns1) (List.Tot.map fst lfuns2) /\
+    tag == func.encode_tag the_tag /\
+    List.Tot.memP (the_tag, lfun) lfuns2
+  )
+  (ensures gfun tag == Some lfun)
+  (decreases List.Tot.length lfuns2)
+let rec mk_global_fun_correct_aux func gfun lfuns1 lfuns2 the_tag lfun tag =
+  match lfuns2 with
+  | [] -> ()
+  | (h_tag, h_sfun)::t -> (
+    eliminate h_tag == the_tag \/ h_tag =!= the_tag returns gfun tag == Some lfun with _. (
+      find_local_fun_wrong_tag func the_tag lfuns1 tag;
+      FStar.Classical.move_requires_3 memP_map fst t (the_tag, lfun)
+    ) and _. (
+      disjointP_move (List.Tot.map fst lfuns1) h_tag (List.Tot.map fst t);
+      List.Tot.map_append fst lfuns1 [(h_tag, h_sfun)];
+      assert_norm(List.Tot.map fst [(h_tag, h_sfun)] == [h_tag]);
+      FStar.Classical.forall_intro (find_local_fun_move func lfuns1 (h_tag, h_sfun) t);
+      mk_global_fun_correct_aux func gfun (lfuns1 @ [(h_tag, h_sfun)]) t the_tag lfun tag
+    )
+  )
+
+val disjointP_nil: #a:Type -> l:list a -> Lemma (disjointP [] l)
+let rec disjointP_nil #a l =
+  match l with
+  | [] -> ()
+  | _::t -> disjointP_nil t
+
+/// Correctness theorem for `mk_global_fun`:
+/// the global function contains all the local functions used to construct it.
+
+val mk_global_fun_correct:
+  func:split_function_input_values -> lfuns:list (func.tag_t & func.local_fun) -> the_tag:func.tag_t -> lfun:func.local_fun ->
+  Lemma
+  (requires
+    List.Tot.no_repeats_p (List.Tot.map fst lfuns) /\
+    List.Tot.memP (the_tag, lfun) lfuns
+  )
+  (ensures has_local_fun func (mk_global_fun func lfuns) (the_tag, lfun))
+let mk_global_fun_correct func lfuns the_tag lfun =
+  reveal_opaque (`%mk_global_fun) (mk_global_fun);
+  introduce
+    forall tagged_data.
+      match func.decode_tagged_data tagged_data with
+      | Some (tag, raw_data) ->
+        tag == func.encode_tag the_tag ==> (func.apply_global_fun (mk_global_fun func lfuns) tagged_data == func.apply_local_fun lfun raw_data)
+      | None -> True
+  with (
+    match func.decode_tagged_data tagged_data with
+    | Some (tag, raw_data) -> (
+      if tag = func.encode_tag the_tag then (
+        disjointP_nil (List.Tot.map fst lfuns);
+        mk_global_fun_correct_aux func (find_local_fun func lfuns) [] lfuns the_tag lfun tag;
+        func.apply_mk_global_fun (mk_global_fun_aux func lfuns) tagged_data
+      ) else ()
+    )
+    | None -> ()
+  )
+
+/// Equivalence theorem for `mk_global_fun`.
+/// This may be useful to lift properties of the local functions
+/// to property on the global function.
+/// (e.g. the function keep the same output when the trace grows.)
+
+val mk_global_fun_eq:
+  func:split_function_input_values -> lfuns:list (func.tag_t & func.local_fun) ->
+  tagged_data:func.tagged_data_t ->
+  Lemma (
+    func.apply_global_fun (mk_global_fun func lfuns) tagged_data == (
+      match func.decode_tagged_data tagged_data with
+      | Some (tag, raw_data) -> (
+        match find_local_fun func lfuns tag with
+        | Some lfun -> func.apply_local_fun lfun raw_data
+        | None -> func.apply_global_fun func.default_global_fun tagged_data
+      )
+      | None -> func.apply_global_fun func.default_global_fun tagged_data
+    )
+  )
+let mk_global_fun_eq func lfuns tagged_data =
+  reveal_opaque (`%mk_global_fun) (mk_global_fun);
+  func.apply_mk_global_fun (mk_global_fun_aux func lfuns) tagged_data
+
+/// If a global function contains some local function,
+/// and the global function input decodes to a tag for this local function,
+/// then the global function is equivalent to the local function on this input.
+
+val local_eq_global_lemma:
+  func:split_function_input_values ->
+  gfun:func.global_fun -> the_tag:func.tag_t -> lfun:func.local_fun ->
+  tagged_data:func.tagged_data_t -> raw_data:func.raw_data_t ->
+  Lemma
+  (requires
+    func.decode_tagged_data tagged_data == Some (func.encode_tag the_tag, raw_data) /\
+    has_local_fun func gfun (the_tag, lfun)
+  )
+  (ensures func.apply_global_fun gfun tagged_data == func.apply_local_fun lfun raw_data)
+let local_eq_global_lemma func gfun the_tag lfun tagged_data raw_data = ()
